changes file structure to make import and exports simple.

src/Relations.dfy
@@ -1,12 +1,6 @@
-
-include "Helpers.dfy"
-
 module Relations { 
     export 
-    reveals Reflexive, AntiSymmetric, Connected, TotalOrdering
-    provides Helpers
-
-    import opened Helpers
+    reveals Reflexive, AntiSymmetric, Connected, TotalOrdering, Transitive, Trichotomous
 
     predicate Reflexive<T(!new)>(R: (T, T) -> bool) 
     {
@@ -27,8 +21,29 @@ module Relations {
     {
     && Reflexive(R)
     && AntiSymmetric(R)
-    && Helpers.Transitive(R)
+    && Transitive(R)
     && Connected(R)
     }  
+
+    /*
+    * To be _trichotomous_ means that for any two `x` and `y`,
+    * EXACTLY one of the following three conditions holds:
+    *   - less(x, y)
+    *   - x == y
+    *   - less(y, x)
+    * Note that being trichotomous implies being irreflexive.
+    */
+
+    predicate Trichotomous<T(!new)>(less: (T, T) -> bool) 
+    {
+        (forall x, y :: less(x, y) || x == y || less(y, x)) &&  // at least one of the three
+        (forall x, y :: less(x, y) && less(y, x) ==> false) &&  // not both of the less's
+        (forall x, y :: less(x, y) ==> x != y)  // not a less and the equality
+    }
+
+    predicate Transitive<T(!new)>(R: (T, T) -> bool) 
+    {
+        forall x, y, z :: R(x, y) && R(y, z) ==> R(x, z)
+    }
 
 }
