src/CompariosRelations.dfy
@@ -1,0 +1,32 @@
+include "Helpers.dfy"
+
+module Relations.ComparisonsRelation { 
+
+    export 
+    reveals Reflexive, AntiSymmetric, Connected, TotalOrdering
+
+    import opened Helpers.Comparison
+
+    predicate Reflexive<T(!new)>(R: (T, T) -> CompResult) 
+    {
+        forall x :: R(x, x)
+    }
+
+    predicate AntiSymmetric<T(!new)>(R: (T, T) -> CompResult) 
+    {
+        forall x, y :: R(x, y) && R(y, x) ==> x == y
+    }
+
+    predicate Connected<T(!new)>(R: (T, T) -> CompResult) 
+    {
+        forall x, y :: R(x, y) || R(y, x)
+    }
+
+    predicate TotalOrdering<T(!new)>(R: (T, T) -> CompResult) 
+    {
+    && Reflexive(R)
+    && AntiSymmetric(R)
+    && Helpers.Transitive(R)
+    && Connected(R)
+    }  
+}
